Superposition_Calculus/Relation_Extra.thy
@@ -2,6 +2,12 @@ theory Relation_Extra
   imports "HOL.Relation"  "Open_Induction.Restricted_Predicates"
 begin
 
+lemma transp_on_empty[simp]: "transp_on {} R"
+  by (auto intro: transp_onI)
+
+lemma asymp_on_empty[simp]: "asymp_on {} R"
+  by (auto intro: asymp_onI)
+
 lemma partition_set_around_element:
   assumes tot: "totalp_on N R" and x_in: "x \<in> N"
   shows "N = {y \<in> N. R y x} \<union> {x} \<union> {y \<in> N. R x y}"
